thy/Primitive_Matchers/Code_Interface.thy
@@ -80,59 +80,96 @@ definition integer_to_16word :: "integer \<Rightarrow> 16 word" where
   "integer_to_16word i \<equiv> nat_to_16word (nat_of_integer i)"
 
 
+
+text{*Example*}
 context
 begin
   (*cool example*)
   lemma "let fw = [''FORWARD'' \<mapsto> [Rule (Match (Src (Ip4AddrNetmask (10,0,0,0) 8))) (Call ''foo'')],
-                         ''foo'' \<mapsto> [Rule (Match (Src (Ip4AddrNetmask (10,128,0,0) 9))) action.Return,
-                                     Rule (Match (Prot (Proto TCP))) action.Accept]
-                         ] in
+                   ''foo'' \<mapsto> [Rule (Match (Src (Ip4AddrNetmask (10,128,0,0) 9))) action.Return,
+                               Rule (Match (Prot (Proto TCP))) action.Accept]
+                   ] in
     let simplfw = to_simple_firewall
-      (upper_closure (optimize_matches abstract_for_simple_firewall (upper_closure (packet_assume_new (unfold_ruleset_FORWARD action.Drop fw)))))
+      (upper_closure (optimize_matches abstract_for_simple_firewall
+        (upper_closure (packet_assume_new (unfold_ruleset_FORWARD action.Drop fw)))))
     in map simple_rule_toString simplfw =
-    [''ACCEPT     tcp  --  10.0.0.0/9            0.0.0.0/0    '', ''DROP     all  --  0.0.0.0/0            0.0.0.0/0    '']" by eval
+    [''ACCEPT     tcp  --  10.0.0.0/9            0.0.0.0/0    '',
+     ''DROP     all  --  0.0.0.0/0            0.0.0.0/0    '']" by eval
   
   (*cooler example*)
-  private definition "cool_example \<equiv> (let fw = [''FORWARD'' \<mapsto> [Rule (Match (Src (Ip4AddrNetmask (10,0,0,0) 8))) (Call ''foo'')],
-                         ''foo'' \<mapsto> [Rule (MatchNot (Match (Src (Ip4AddrNetmask (10,0,0,0) 9)))) action.Drop,
-                                     Rule (Match (Prot (Proto TCP))) action.Accept]
-                         ] in
-    to_simple_firewall (upper_closure (optimize_matches abstract_for_simple_firewall (upper_closure (packet_assume_new (unfold_ruleset_FORWARD action.Drop fw))))))"
+  private definition "cool_example \<equiv> (let fw = 
+                [''FORWARD'' \<mapsto> [Rule (Match (Src (Ip4AddrNetmask (10,0,0,0) 8))) (Call ''foo'')],
+                 ''foo'' \<mapsto> [Rule (MatchNot (Match (Src (Ip4AddrNetmask (10,0,0,0) 9)))) action.Drop,
+                             Rule (Match (Prot (Proto TCP))) action.Accept]
+                 ] in
+    to_simple_firewall (upper_closure (optimize_matches abstract_for_simple_firewall
+                          (upper_closure (packet_assume_new (unfold_ruleset_FORWARD action.Drop fw))))))"
   lemma " map simple_rule_toString cool_example =
-    [''DROP     all  --  10.128.0.0/9            0.0.0.0/0    '', ''ACCEPT     tcp  --  10.0.0.0/8            0.0.0.0/0    '',
-    ''DROP     all  --  0.0.0.0/0            0.0.0.0/0    '']"
+    [''DROP     all  --  10.128.0.0/9            0.0.0.0/0    '',
+     ''ACCEPT     tcp  --  10.0.0.0/8            0.0.0.0/0    '',
+     ''DROP     all  --  0.0.0.0/0            0.0.0.0/0    '']"
   by eval
   
-  value[code] "map ipv4addr_wordinterval_toString (getParts cool_example)"
+  lemma "map ipv4addr_wordinterval_toString (getParts cool_example) =
+    [''{10.128.0.0 .. 10.255.255.255}'',
+     ''{10.0.0.0 .. 10.127.255.255}'',
+     ''{0.0.0.0 .. 9.255.255.255} u {11.0.0.0 .. 255.255.255.255}'']" by eval
   
-  value[code] "map ipv4addr_wordinterval_toString (build_ip_partition parts_connection_ssh cool_example)"
+  lemma "map ipv4addr_wordinterval_toString (build_ip_partition parts_connection_ssh cool_example) =
+    [''{0.0.0.0 .. 9.255.255.255} u {10.128.0.0 .. 255.255.255.255}'',
+     ''{10.0.0.0 .. 10.127.255.255}'']" by eval
   
   (*it is not minimal if we allow to further compress the node definitions?
   the receiver nodes could be combined to UNIV
   But minimal for a symmetric matrix*)
-  value[code] "access_matrix_pretty parts_connection_ssh cool_example"
+  lemma "access_matrix_pretty parts_connection_ssh cool_example =
+    ([(''Nodes'', '':''),
+      (''0.0.0.0'', ''{0.0.0.0 .. 9.255.255.255} u {10.128.0.0 .. 255.255.255.255}''),
+      (''10.0.0.0'', ''{10.0.0.0 .. 10.127.255.255}'')],
+     [(''Edges'', '':''),
+      (''10.0.0.0'', ''0.0.0.0''),
+      (''10.0.0.0'', ''10.0.0.0'')])" by eval
 end
-
-
 context
 begin
-  (*prob look at dst also*)
+  (*now with a destination IP*)
   private definition "cool_example2 \<equiv> (let fw =
     [''FORWARD'' \<mapsto> [Rule (Match (Src (Ip4AddrNetmask (10,0,0,0) 8))) (Call ''foo'')],
      ''foo'' \<mapsto> [Rule (MatchNot (Match (Src (Ip4AddrNetmask (10,0,0,0) 9)))) action.Drop,
                  Rule (MatchAnd (Match (Prot (Proto TCP))) (Match (Dst (Ip4AddrNetmask (10,0,0,42) 32)))) action.Accept]
-                         ] in
-    to_simple_firewall (upper_closure (optimize_matches abstract_for_simple_firewall (upper_closure (packet_assume_new (unfold_ruleset_FORWARD action.Drop fw))))))"
-  value[code] "map simple_rule_toString cool_example2"
+                ] in
+    to_simple_firewall (upper_closure (optimize_matches abstract_for_simple_firewall
+                          (upper_closure (packet_assume_new (unfold_ruleset_FORWARD action.Drop fw))))))"
+  lemma "map simple_rule_toString cool_example2 =
+    [''DROP     all  --  10.128.0.0/9            0.0.0.0/0    '',
+     ''ACCEPT     tcp  --  10.0.0.0/8            10.0.0.42/32    '',
+     ''DROP     all  --  0.0.0.0/0            0.0.0.0/0    '']" by eval
   
-  value[code] "map ipv4addr_wordinterval_toString (getParts cool_example2)"
+  (*not minimal*)
+  lemma "map ipv4addr_wordinterval_toString (getParts cool_example2) =
+    [''{10.128.0.0 .. 10.255.255.255}'', ''10.0.0.42'',
+     ''{10.0.0.0 .. 10.0.0.41} u {10.0.0.43 .. 10.127.255.255}'',
+     ''{0.0.0.0 .. 9.255.255.255} u {11.0.0.0 .. 255.255.255.255}'']" by eval
   
-  value[code] "map ipv4addr_wordinterval_toString (build_ip_partition parts_connection_ssh cool_example2)"
+  lemma "map ipv4addr_wordinterval_toString (build_ip_partition parts_connection_ssh cool_example2) =
+    [''{0.0.0.0 .. 9.255.255.255} u {10.128.0.0 .. 255.255.255.255}'', ''10.0.0.42'',
+     ''{10.0.0.0 .. 10.0.0.41} u {10.0.0.43 .. 10.127.255.255}'']" by eval
   
-  value[code] "access_matrix_pretty parts_connection_ssh cool_example2"
+  lemma "access_matrix_pretty parts_connection_ssh cool_example2 =
+    ([(''Nodes'', '':''),
+      (''0.0.0.0'', ''{0.0.0.0 .. 9.255.255.255} u {10.128.0.0 .. 255.255.255.255}''),
+      (''10.0.0.42'', ''10.0.0.42''),
+      (''10.0.0.0'', ''{10.0.0.0 .. 10.0.0.41} u {10.0.0.43 .. 10.127.255.255}'')
+     ],
+     [(''Edges'', '':''),
+      (''10.0.0.42'', ''10.0.0.42''),
+      (''10.0.0.0'', ''10.0.0.42'')
+     ])" by eval
   end
 
 
+
+(*currently unused and unverifed. may be needed for future use*)
 definition prefix_to_strange_inverse_cisco_mask:: "nat \<Rightarrow> (nat \<times> nat \<times> nat \<times> nat)" where
  "prefix_to_strange_inverse_cisco_mask n \<equiv> dotdecimal_of_ipv4addr ( (NOT (((mask n)::ipv4addr) << (32 - n))) )"
 lemma "prefix_to_strange_inverse_cisco_mask 8 = (0, 255, 255, 255)" by eval
@@ -142,7 +179,7 @@ lemma "prefix_to_strange_inverse_cisco_mask 32 = (0, 0, 0, 0)" by eval
 
 
 
-
+(*TODO: theorem!*)
 definition "to_simple_firewall_without_interfaces ipassmt rs \<equiv>
     to_simple_firewall
     (upper_closure
